ver2/concrete_interpreter.v
@@ -33,10 +33,10 @@ Definition push_c (v : EVMWord) (st : state) (ops : stack_op_instr_map) : option
   | Some stk' => Some (set_stack_st st stk')
   end.
 
-Definition pushtag_c (v : N) (st : state) (ops : stack_op_instr_map) : option state :=
+Definition pushtag_c (v1 v2 : N) (st : state) (ops : stack_op_instr_map) : option state :=
   let stk := get_stack_st st in
   let tags := (get_tags_ctx (get_context_st st)) in
-  let v' := tags v in
+  let v' := tags v1 v2 in
   match push v' stk with
   | None => None
   | Some stk' => Some (set_stack_st st stk')
@@ -179,7 +179,7 @@ Definition exec_stack_op_intsr_c (label : stack_op_instr) (st : state) (ops : st
 Definition evm_exec_instr_c (inst : instr) (st: state) (ops : stack_op_instr_map) : option state :=
   match inst with
   | PUSH size v => push_c (NToWord EVMWordSize v) st ops
-  | PUSHTAG v => pushtag_c v st ops
+  | PUSHTAG cat v => pushtag_c cat v st ops
   | POP => pop_c st ops
   | DUP k => dup_c k st ops
   | SWAP k => swap_c k st ops
