ver2/symbolic_state_eval.v
@@ -56,8 +56,8 @@ Fixpoint eval_sstack_val' (d : nat) (sv : sstack_val) (stk : stack) (mem: memory
           | SymBasicVal (FreshVar _) => None
 
           (* PUSHTAG *)
-          | SymPUSHTAG v =>
-              let tags := (get_tags_ctx ctx) in Some (tags v)
+          | SymPUSHTAG cat v =>
+              let tags := (get_tags_ctx ctx) in Some (tags cat v)
 
           (* stack operation instruction: we evaluate the argument
              recursively and then evaluate the corresponding operation *)
